modernized arm strlen proof

strlen_arm_proofs.v
@@ -44,1329 +44,287 @@ Proof.
   prove_noassign.
 Qed.
 
-Tactic Notation "destN" constr(n) "until" tactic(T) "eqn" ":" ident(H) :=
-  let p := fresh n in
-  destruct n as [|p] eqn:H;
-  [ try solve [T]
-  | repeat first [ solve[T] | destruct p as [p|p|] ] ].
+Definition nilfree (m:addr->N) (p:addr) (k:N) :=
+  forall i, i < k -> m (p⊕i) <> 0.
 
-(* Tactic: focus_addr H n
-   Shelve all goals except the goal in which hypothesis H has the form (H: _ = n).
-   This retrieves the subgoal for address n from a sea of arbitrarily ordered goals.
-   Use vernacular command "Unshelve" to pull back all the shelved goals afterward. *)
-Tactic Notation "focus_addr" hyp(H) constr(n) :=
-  match type of H with _ = n => idtac | _ => shelve end.
-
-Lemma N_lt_m:
-  forall n m, n < m -> n = m-1 \/ n < m-1.
-Proof.
-  intros. apply N.lt_le_pred in H.
-  rewrite N.pred_sub in H. apply N.le_lteq in H.
-  destruct H; [right | left]; assumption.
-Qed.
-
-Corollary N_lt_4 : forall n, n < 4 -> n = 0 \/ n = 1 \/ n = 2 \/ n = 3.
-Proof.
-  intros.
-  do 4 try (apply N_lt_m in H; destruct H).
-  all: repeat (try (try left; assumption); try right).
-  apply N.nlt_0_r in H; inversion H.
-Qed.
-
-Lemma if_true : forall (A:Type) (a1 a2:A) b,
-  a1 ≠ a2 ->
-  b = true <-> (if b then a1 else a2) = a1.
-Proof.
-  intros. split.
-    intros.
-    destruct b; [ reflexivity | discriminate ].
-  intros. destruct b. reflexivity. subst a2. contradiction.
-Qed.
-
-Lemma if_false : forall (A:Type) (a1 a2:A) b,
-  a1 ≠ a2 ->
-  b = false <-> (if b then a1 else a2) = a2.
-Proof.
-  intros. split.
-    intros.
-    destruct b; [ discriminate | reflexivity ].
-  intros. destruct b; [ contradiction | reflexivity].
-Qed.
-
-Lemma if_neq_then : forall (A:Type) (a1 a2:A) (b:bool),
-  a1 ≠ a2 ->
-  (if b then a1 else a2) ≠ a1 <-> (if b then a1 else a2) = a2.
-Proof.
-  split; intros.
-  destruct b. contradiction. reflexivity.
-  destruct b. contradiction. intros H1. subst a2. contradiction.
-Qed.
-
-Lemma if_neq_else : forall (A:Type) (a1 a2:A) (b:bool),
-  a1 ≠ a2 ->
-  (if b then a1 else a2) ≠ a2 <-> (if b then a1 else a2) = a1.
-Proof.
-  split; intros.
-  destruct b. reflexivity. contradiction.
-  destruct b. assumption. rewrite H0 in H. contradiction.
-Qed.
-
-Lemma pos_le_0_1 : forall a b,
-  N.pos a <= N.pos b ->
-  N.pos a~0 <= N.pos b~1.
-Proof.
-  intros.
-  replace (N.pos a~0) with (N.shiftl (N.pos a) 1) by reflexivity.
-  replace (N.pos b~1) with ((N.shiftl (N.pos b) 1) + 1) by reflexivity.
-  repeat rewrite N.shiftl_mul_pow2; replace (2^1) with 2 by reflexivity.
-  apply N.le_trans with (N.pos b * 2).
-  apply N.mul_le_mono_r; assumption.
-  apply N.le_add_r.
-Qed.
-
-Lemma pos_le_1_1 : forall a b,
-  N.pos a <= N.pos b ->
-  N.pos a~1 <= N.pos b~1.
-Proof.
-  intros.
-  replace (N.pos a~1) with ((N.shiftl (N.pos a) 1) + 1) by reflexivity.
-  replace (N.pos b~1) with ((N.shiftl (N.pos b) 1) + 1) by reflexivity.
-  apply N.add_le_mono_r. repeat rewrite N.shiftl_mul_pow2. 
-  replace (2^1) with 2 by reflexivity. apply N.mul_le_mono_r. assumption.
-Qed.
-
-Lemma pos_le_0_0 : forall a b,
-  N.pos a <= N.pos b ->
-  N.pos a~0 <= N.pos b~0.
-Proof.
-  intros.
-  replace (N.pos a~0) with (N.shiftl (N.pos a) 1) by reflexivity.
-  replace (N.pos b~0) with (N.shiftl (N.pos b) 1) by reflexivity.
-  repeat rewrite N.shiftl_mul_pow2; replace (2^1) with 2 by reflexivity.
-  apply N.mul_le_mono_r. assumption.
-Qed.
-
-Theorem and_le_l : forall a b, a .& b <= a.
-Proof.
-  intros.
-  destruct a, b.
-  1-3: discriminate 1.
-  revert dependent p0. induction p; intros.
-  3: simpl; destruct p0; discriminate 1.
-  simpl. destruct p0.
-    destruct (Pos.land p p0) eqn:Hand. discriminate 1.
-      simpl. apply pos_le_1_1. rewrite <- Hand. apply IHp.
-    destruct (Pos.land p p0) eqn:Hand. discriminate 1.
-      simpl. apply pos_le_0_1. rewrite <- Hand. apply IHp.
-  discriminate 1.
-  simpl. destruct p0.
-    destruct (Pos.land p p0) eqn:Hand. discriminate 1.
-      simpl. apply pos_le_0_0. rewrite <- Hand. apply IHp.
-    destruct (Pos.land p p0) eqn:Hand. discriminate 1.
-      simpl. apply pos_le_0_0. rewrite <- Hand. apply IHp.
-  discriminate 1.
-Qed.
-
-Theorem and_le_r : forall a b, a .& b <= b.
-Proof.
-  intros. rewrite N.land_comm. apply and_le_l.
-Qed.
-
-Lemma mod_and_3 : forall a, a mod 2 ^ 2 = a .& 3.
-Proof.
-  intros. rewrite <- N.land_ones. reflexivity.
-Qed.
-
-Lemma n_lt_mul : forall n m,
-  m > 0 ->
-  n <= n * m.
-Proof.
-  intros.
-  destruct m. discriminate. clear H.
-  induction p.
-    replace (N.pos p~1) with (2*N.pos p + 1) by reflexivity.
-    rewrite N.mul_add_distr_l, N.mul_1_r, N.add_comm. 
-    apply N.le_add_r.
-
-    replace (N.pos p~0) with (2*N.pos p) by reflexivity.
-    rewrite N.mul_comm, N.mul_shuffle0.
-    apply N.le_trans with (n*N.pos p). assumption.
-    rewrite <- N.mul_assoc. replace 2 with (1+1) by reflexivity.
-    rewrite N.mul_add_distr_r, N.mul_1_l.
-    apply N.le_add_r.
-
-    rewrite N.mul_1_r. apply N.le_refl. 
-Qed.
-
-Lemma N_land_lo_hi_eq0 : forall a b,
-  a < 2 ^ 8 ->
-  a .& (b << 8) = 0.
-Proof.
-  intros.
-  destruct a,b; try reflexivity.
-  do 8 (destruct p; try reflexivity).
-  all: destruct p; inversion H.
-Qed.
-
-Lemma N_add_lnot_land_3 : forall a,
-  a < 2^32 ->
-  (a .& N.lnot 3 32) + (a .& 3) = a.
-Proof.
-  intros. destruct a. reflexivity.
-  destruct p; try reflexivity;
-  destruct p; try reflexivity; simpl.
-  1: replace (N.pos p~1~1) with ((Pos.Ndouble (Pos.Ndouble (N.pos p))) + 3)
-       by reflexivity.
-  2: replace (N.pos p~0~1) with ((Pos.Ndouble (Pos.Ndouble (N.pos p))) + 1)
-       by reflexivity.
-  3: replace (N.pos p~1~0) with ((Pos.Ndouble (Pos.Ndouble (N.pos p))) + 2)
-       by reflexivity.
-  4: replace (N.pos p~0~0) with ((Pos.Ndouble (Pos.Ndouble (N.pos p))) + 0)
-       by reflexivity.
-  all: apply N.add_cancel_r, f_equal, f_equal.
-  all: rewrite <- N.mod_small with (b:=2^30), <- N.land_ones;
-       try reflexivity.
-  all: apply N.mul_lt_mono_pos_l with (p:=4); try reflexivity.
-  all: replace (4*2^30) with (2^32) by reflexivity.
-  1: replace (N.pos p~1~1) with (4 * (N.pos p) + 3) in H by reflexivity.
-  2: replace (N.pos p~0~1) with (4 * (N.pos p) + 1) in H by reflexivity.
-  3: replace (N.pos p~1~0) with (4 * (N.pos p) + 2) in H by reflexivity.
-  4: replace (N.pos p~0~0) with (4 * (N.pos p) + 0) in H by reflexivity.
-  4: assumption.
-  all: eapply N.lt_trans; [apply N.lt_add_pos_r|eassumption]; reflexivity.
-Qed.
-
-Lemma mod_n_le: forall a b n,
-  n ≠ 0 ->
-  a mod n = b ->
-  b <= a.
-Proof.
-  intros. rewrite <- H0. apply N.mod_le. assumption.
-Qed.
-
-Lemma and_mod_eq: forall a,
-  a < 2^32 ->
-  a .& N.lnot 3 32 = a - (a .& 3).
-Proof.
-  intros. symmetry.
-  replace (a - (a .& 3)) with ((a .& N.lnot 3 32) + (a .& 3) - (a .& 3)).
-  2:{ rewrite N_add_lnot_land_3 at 1. reflexivity. assumption. }
-  rewrite N.add_sub. reflexivity.
-Qed.
-
-Theorem mem_ff_gt0 : forall m a,
-  welltyped_memory m ->
-  m Ⓓ[a] .& 255 > 0 ->
-  m a > 0.
-Proof.
-  intros m a WTM H.
-  simpl in H. unfold getmem_little, Mb, mem_bits in H. simpl in H.
-  rewrite N.land_lor_distr_l, N.lor_0_r in H.
-  replace ((m (N.succ a) 
-        .| (m (N.succ (N.succ a)) 
-        .| (m (N.succ (N.succ (N.succ a))) << 8) << 8) << 8) .& 255)
-    with 0 in H.
-  rewrite N.lor_0_r in H. replace 255 with (N.ones 8) in H by reflexivity.
-  rewrite N.land_ones, N.mod_small in H by apply WTM.
-  assumption.
-  clear H. symmetry.
-  remember (m (N.succ a) 
-        .| (m (N.succ (N.succ a)) 
-        .| (m (N.succ (N.succ (N.succ a))) << 8) << 8))
-  as z.
-  destruct z; try reflexivity.
-Qed.
-
-Theorem mem_ff00_gt0 : forall m a,
-  welltyped_memory m ->
-  m Ⓓ[a] .& 65280 > 0 ->
-  m (a+1) > 0.
-Proof.
-  intros m a WTM H.
-  simpl in H. unfold getmem_little, Mb, mem_bits in H. simpl in H.
-  rewrite N.land_lor_distr_l, N.lor_0_r in H.
-  replace (m a .& 65280) with 0 in H.
-  replace 65280 with (255 << 8) in H by reflexivity.
-  rewrite N.lor_0_l, <- N.shiftl_land, N.shiftl_mul_pow2 in H.
-  replace 0 with (0*2^8) in H by reflexivity.
-  apply N.gt_lt, N.mul_lt_mono_pos_r, N.lt_gt in H.
-  rewrite N.land_lor_distr_l in H.
-  replace ((m (N.succ (N.succ a)) 
-         .| (m (N.succ (N.succ (N.succ a))) << 8) << 8) .& 255)
-    with 0 in H.
-  rewrite N.lor_0_r in H. replace 255 with (N.ones 8) in H by reflexivity.
-  rewrite N.land_ones, N.mod_small in H by apply WTM.
-  rewrite N.add_1_r.
-  assumption.
-  clear H. symmetry.
-  remember (m (N.succ (N.succ a)) 
-         .| (m (N.succ (N.succ (N.succ a))) << 8))
-  as z.
-  destruct z; try reflexivity.
-  reflexivity.
-  remember (m a) as z. destruct z; try reflexivity.
-  symmetry. replace 65280 with (255 << 8) by reflexivity.
-  apply N_land_lo_hi_eq0. rewrite Heqz. apply WTM.
-Qed.
-
-Theorem mem_ff0000_gt0 : forall m a,
-  welltyped_memory m ->
-  m Ⓓ[a] .& 16711680 > 0 ->
-  m (a+2) > 0.
-Proof.
-  intros m a WTM H.
-  simpl in H. unfold getmem_little, Mb, mem_bits in H. simpl in H.
-  rewrite N.land_lor_distr_l, N.lor_0_r in H.
-  replace (m a .& 16711680) with 0 in H.
-  replace 16711680 with (255 << 8 << 8) in H by reflexivity.
-  rewrite N.lor_0_l, <- N.shiftl_land, N.shiftl_mul_pow2 in H.
-  replace 0 with (0*2^8) in H by reflexivity.
-  apply N.gt_lt, N.mul_lt_mono_pos_r, N.lt_gt in H; try reflexivity.
-  rewrite N.land_lor_distr_l in H.
-  replace (m (N.succ a) .& (255 << 8)) with 0 in H.
-  rewrite N.lor_0_l, <- N.shiftl_land, N.shiftl_mul_pow2 in H.
-  replace 0 with (0*2^8) in H by reflexivity.
-  apply N.gt_lt, N.mul_lt_mono_pos_r, N.lt_gt in H; try reflexivity.
-  rewrite N.land_lor_distr_l in H.
-  replace ((m (N.succ (N.succ (N.succ a))) << 8) .& 255) with 0 in H.
-  rewrite N.lor_0_r in H. replace 255 with (N.ones 8) in H by reflexivity.
-  rewrite N.land_ones, N.mod_small in H by apply WTM.
-  replace (a+2) with (a+(1+1)) by reflexivity.
-  rewrite N.add_assoc, N.add_1_r, N.add_1_r.
-  assumption.
-  all: clear H; symmetry.
-  remember (m (N.succ (N.succ (N.succ a)))) as z.
-  destruct z; try reflexivity.
-  apply N_land_lo_hi_eq0. apply WTM.
-  replace 16711680 with (65280 << 8) by reflexivity.
-  apply N_land_lo_hi_eq0. apply WTM.
-Qed.
-
-Theorem mem_ff000000_gt0 : forall m a,
-  welltyped_memory m ->
-  m Ⓓ[a] .& 4278190080 > 0 ->
-  m (a+3) > 0.
-Proof.
-  intros m a WTM H.
-  simpl in H. unfold getmem_little, Mb, mem_bits in H. simpl in H.
-  rewrite N.land_lor_distr_l, N.lor_0_r in H.
-  replace (m a .& 4278190080) with 0 in H.
-  replace 4278190080 with (255 << 8 << 8 << 8) in H by reflexivity.
-  rewrite N.lor_0_l, <- N.shiftl_land, N.shiftl_mul_pow2 in H.
-  replace 0 with (0*2^8) in H by reflexivity.
-  apply N.gt_lt, N.mul_lt_mono_pos_r, N.lt_gt in H; try reflexivity.
-  rewrite N.land_lor_distr_l in H.
-  replace (m (N.succ a) .& (255 << 8 << 8)) with 0 in H.
-  rewrite N.lor_0_l, <- N.shiftl_land, N.shiftl_mul_pow2 in H.
-  replace 0 with (0*2^8) in H by reflexivity.
-  apply N.gt_lt, N.mul_lt_mono_pos_r, N.lt_gt in H; try reflexivity.
-  rewrite N.land_lor_distr_l in H.
-  replace (m (N.succ (N.succ a)) .& (255 << 8)) with 0 in H.
-  rewrite N.lor_0_l in H. replace 255 with (N.ones 8) in H by reflexivity.
-  rewrite <- N.shiftl_land, N.land_ones, N.mod_small in H by apply WTM.
-  replace (a+3) with (a+(1+1+1)) by reflexivity.
-  rewrite N.add_assoc, N.add_assoc, N.add_1_r, N.add_1_r, N.add_1_r.
-  replace 0 with (0*2^8) in H by reflexivity.
-  rewrite N.shiftl_mul_pow2 in H.
-  apply N.gt_lt, N.mul_lt_mono_pos_r, N.lt_gt in H; try reflexivity.
-  assumption.
-  all: clear H; symmetry.
-  apply N_land_lo_hi_eq0. apply WTM.
-  apply N_land_lo_hi_eq0. apply WTM.
-  replace 4278190080 with (16711680 << 8) by reflexivity.
-  apply N_land_lo_hi_eq0. apply WTM.
-Qed.
-
-Theorem mem_ff_eq0 : forall m a,
-  welltyped_memory m ->
-  m Ⓓ[a] .& 255 = 0 ->
-  m a = 0.
-Proof.
-  intros m a WTM H.
-  simpl in H. unfold getmem_little, Mb, mem_bits in H. simpl in H.
-  rewrite N.land_lor_distr_l in H. apply N.lor_eq_0_l in H.
-  replace 255 with (N.ones 8) in H by reflexivity.
-  rewrite N.land_ones, N.mod_small in H by apply WTM.
-  assumption.
-Qed.
-
-Theorem mem_ff00_eq0 : forall m a,
-  welltyped_memory m ->
-  m Ⓓ[a] .& 65280 = 0 ->
-  m (a+1) = 0.
-Proof.
-  intros m a WTM H.
-  simpl in H. unfold getmem_little, Mb, mem_bits in H. simpl in H.
-  rewrite N.land_lor_distr_l, N.lor_0_r in H. apply N.lor_eq_0_iff in H.
-  destruct H as [_ H].
-  replace 65280 with (255 << 8) in H by reflexivity.
-  rewrite <- N.shiftl_land, N.shiftl_mul_pow2 in H.
-  replace 0 with (0*2^8) in H by reflexivity.
-  apply N.mul_cancel_r in H; try discriminate.
-  rewrite N.land_lor_distr_l in H. apply N.lor_eq_0_l in H.
-  replace 255 with (N.ones 8) in H by reflexivity.
-  rewrite N.land_ones, N.mod_small in H by apply WTM.
-  rewrite N.add_1_r.
-  assumption.
-Qed.
-
-Theorem mem_ff0000_eq0 : forall m a,
-  welltyped_memory m ->
-  m Ⓓ[a] .& 16711680 = 0 ->
-  m (a+2) = 0.
-Proof.
-  intros m a WTM H.
-  simpl in H. unfold getmem_little, Mb, mem_bits in H. simpl in H.
-  rewrite N.land_lor_distr_l, N.lor_0_r in H. apply N.lor_eq_0_iff in H.
-  destruct H as [_ H].
-  replace 16711680 with (255 << 8 << 8) in H by reflexivity.
-  rewrite <- N.shiftl_land, N.shiftl_mul_pow2 in H.
-  replace 0 with (0*2^8) in H by reflexivity.
-  apply N.mul_cancel_r in H; try discriminate.
-  rewrite N.land_lor_distr_l in H. apply N.lor_eq_0_iff in H.
-  destruct H as [_ H].
-  rewrite <- N.shiftl_land, N.shiftl_mul_pow2 in H.
-  replace 0 with (0*2^8) in H by reflexivity.
-  apply N.mul_cancel_r in H; try discriminate.
-  rewrite N.land_lor_distr_l in H. apply N.lor_eq_0_l in H.
-  replace 255 with (N.ones 8) in H by reflexivity.
-  rewrite N.land_ones, N.mod_small in H by apply WTM.
-  replace 2 with (1+1) by reflexivity.
-  rewrite N.add_assoc, N.add_1_r, N.add_1_r.
-  assumption.
-Qed.
-
-Theorem mem_ff000000_eq0 : forall m a,
-  welltyped_memory m ->
-  m Ⓓ[a] .& 4278190080 = 0 ->
-  m (a+3) = 0.
-Proof.
-  intros m a WTM H.
-  simpl in H. unfold getmem_little, Mb, mem_bits in H. simpl in H.
-  rewrite N.land_lor_distr_l, N.lor_0_r in H. apply N.lor_eq_0_iff in H.
-  destruct H as [_ H].
-  replace 4278190080 with (255 << 8 << 8 << 8) in H by reflexivity.
-  rewrite <- N.shiftl_land, N.shiftl_mul_pow2 in H.
-  replace 0 with (0*2^8) in H by reflexivity.
-  apply N.mul_cancel_r in H; try discriminate.
-  rewrite N.land_lor_distr_l in H. apply N.lor_eq_0_iff in H.
-  destruct H as [_ H].
-  rewrite <- N.shiftl_land, N.shiftl_mul_pow2 in H.
-  replace 0 with (0*2^8) in H by reflexivity.
-  apply N.mul_cancel_r in H; try discriminate.
-  rewrite N.land_lor_distr_l in H. apply N.lor_eq_0_iff in H.
-  destruct H as [_ H].
-  rewrite <- N.shiftl_land, N.shiftl_mul_pow2 in H.
-  replace 0 with (0*2^8) in H by reflexivity.
-  apply N.mul_cancel_r in H; try discriminate.
-  replace 255 with (N.ones 8) in H by reflexivity.
-  rewrite N.land_ones, N.mod_small in H by apply WTM.
-  replace 3 with (1+1+1) by reflexivity.
-  rewrite N.add_assoc, N.add_assoc, N.add_1_r, N.add_1_r, N.add_1_r.
-  assumption.
-Qed.
-
-Definition nilfree (m:addr->N) (start:addr) (len:N) :=
-  forall i, i < len -> m (start+i) > 0.
-
-Theorem nilfree_split : forall m a j k,
-  nilfree m a j ->
-  nilfree m (a+j) k ->
-  nilfree m a (j+k).
-Proof.
-  unfold nilfree. intros.
-  assert (Hlt: j <= i \/ i < j) by apply N.le_gt_cases.
-  inversion Hlt. 2: apply H, H2.
-  specialize H0 with (i-j).
-  rewrite N.add_sub_assoc in H0 by assumption.
-  rewrite N.add_sub_swap, N.add_sub in H0.
-  apply H0. clear H H0 Hlt.
-  assert (i <= j + k) by (apply N.lt_le_incl; assumption).
-  assert (∃ x, i = j + x). exists (i-j).
-  rewrite N.add_sub_assoc, N.add_comm, N.add_sub by assumption; reflexivity.
-  destruct H0. rewrite H0, N.add_comm, N.add_sub.
-  rewrite H0, <- N.add_lt_mono_l in H1; assumption.
-  rewrite N.add_comm. apply N.le_add_r.
-Qed.
-
-Definition nilfree_dword (n:N) : N :=
-  if N.eqb (n .& 255) 0 then 0 else
-  if N.eqb (n .& 65280) 0 then 1 else
-  if N.eqb (n .& 16711680) 0 then 2 else
-  if N.eqb (n .& 4278190080) 0 then 3 else 4.
-
-Definition loop_inv (n _r0 r0 r1 r2:N) (m:addr->N) :=
-  ((n ≠ 0 /\ r2 = m Ⓓ[r1 - 4] /\ nilfree m _r0 r0 
-          /\ r0 + 4 <= r1 /\ r0 = 4*n - (_r0 .& 3)) \/
-   (n = 0 /\ ((_r0 mod 4 = 0 /\ r2 = m Ⓓ[r1 - 4]) \/
-              (_r0 mod 4 = 1 /\ r2 = m Ⓓ[r1 - 4] .| 255) \/
-              (_r0 mod 4 = 2 /\ r2 = m Ⓓ[r1 - 4] .| 255 .| 65280) \/
-              (_r0 mod 4 = 3 /\ r2 = m Ⓓ[r1 - 4] .| 255 .| 65280 .| 16711680))
-          /\ r0 = (2^32 ⊖ (_r0 .& 3)))).
-
-Definition strlen_invs (m:addr->N) (_r0:N) (a:addr) (s:store) :=
+Definition strlen_invs (m:addr->N) (p a:addr) (s:store) :=
   match a with
-  | 0 => Some (s R_R0 = Ⓓ_r0)
-  | 40 => Some (∃ n r0 r1 r2,
-                   s R_R0 = Ⓓr0 /\ s R_R1 = Ⓓr1 /\ s R_R2 = Ⓓr2
-                /\ r1 = (_r0 .& N.lnot 3 32) + 4 * (n + 1)
-                /\ r1 < 2^32
-                /\ loop_inv n _r0 r0 r1 r2 m)
-  | 68 => Some (∃ n r0 r1 r2,
-                   s R_R0 = Ⓓr0 /\ s R_R1 = Ⓓr1 /\ s R_R2 = Ⓓr2
-                /\ r1 = (_r0 .& N.lnot 3 32) + 4 * (n + 1)
-                /\ r1 < 2^32
-                /\ loop_inv n _r0 r0 r1 r2 m
-                /\ nilfree_dword r2 < 4)
-  | 92 => Some (∃ r0,
-                   s R_R0 = Ⓓr0 
-                /\ nilfree m _r0 r0
-                /\ m (_r0 + r0) = 0)
+  | 0 => Some (s R_R0 = Ⓓp)
+  | 40 => Some (∃ k, s R_R0 = Ⓓ(2^32 - p mod 4 ⊕ 4*k) /\
+                     s R_R1 = Ⓓ(p - p mod 4 ⊕ 4*N.succ k) /\
+                     s R_R2 = Ⓓ match k with N0 => m Ⓓ[ p - p mod 4 ] .| N.ones (p mod 4 * 8)
+                                           | _ => m Ⓓ[ p - p mod 4 ⊕ 4*k ] end /\
+                     nilfree m p (4*k - p mod 4))
   | _ => None
   end.
 
-Definition strlen_post (mem:addr->N) (_r0:N) (_:exit) (s:store) :=
-  exists r0, s R_R0 = VaN r0 32 /\
-             mem (_r0 + r0) = 0 /\
-             forall i, i < r0 -> mem (_r0+i) > 0.
+Definition strlen_post (m:addr->N) (p:addr) (_:exit) (s:store) :=
+  ∃ k, s R_R0 = Ⓓk /\ nilfree m p k /\ m (p⊕k) = 0.
 
-Definition strlen_invset (mem:addr->N) (_r0:N) :=
-  invs (strlen_invs mem _r0) (strlen_post mem _r0).
+Definition strlen_invset (m:addr->N) (p:addr) :=
+  invs (strlen_invs m p) (strlen_post m p).
+
+Lemma modsubcmp:
+  forall x y z, y <= x -> (x - y =? z) = (x =? z+y).
+Proof.
+  intros. destruct (x =? z + y) eqn:H1.
+    apply Neqb_ok in H1. subst. rewrite N.add_sub. apply N.eqb_refl.
+    apply N.eqb_neq. intro H2. eapply N.eqb_neq. exact H1. subst. rewrite N.sub_add by exact H. reflexivity.
+Qed.
+
+Lemma ldiff_sub:
+  forall x y, N.ldiff x y = x - (x .& y).
+Proof.
+  intros. rewrite N.sub_nocarry_ldiff; apply N.bits_inj; intro n;
+  rewrite 2?N.ldiff_spec, N.land_spec, 1?N.bits_0;
+  repeat destruct (N.testbit _ _); reflexivity.
+Qed.
+
+Lemma nilfree_mod:
+  forall m p a x, nilfree m p a -> nilfree m p (a mod 2^x).
+Proof.
+  intros. intros i LT. apply H. eapply N.lt_le_trans. exact LT.
+  apply N.mod_le. apply N.pow_nonzero. discriminate.
+Qed.
+
+Lemma index_bound:
+  forall p k j, p < 2^32 -> j < 4 -> p - p mod 4 ⊕ 4*k + j < 2^32.
+Proof.
+  intros. change (2^32) with (4*2^30) at 1. change (2^32) with (4*N.pred (2^30) + 4).
+  rewrite (N.div_mod' p 4) at 1.
+  rewrite N.add_sub, <- N.mul_add_distr_l, N.mul_mod_distr_l by discriminate.
+    apply N.add_le_lt_mono; [|assumption].
+    apply N.mul_le_mono_l, N.lt_le_pred, N.mod_lt. discriminate.
+Qed.
+
+Lemma getbyte_lor:
+  forall i x len m a (WTM: welltyped_memory m),
+  i<len -> (getmem LittleE len m a .| x) .& (N.ones 8 << (8*i)) = (m (a+i) .| ((x >> (8*i)) mod 2^8)) << (8*i).
+Proof.
+  intros.
+  rewrite <- (N.sub_add i len), N.add_comm, getmem_split by apply N.lt_le_incl, H.
+  rewrite <- (recompose_bytes (8*i) x) at 1.
+  rewrite N.lor_assoc, <- (N.lor_assoc (getmem _ i m a)), (N.lor_comm _ (_ mod _)), N.lor_assoc, <- N.lor_assoc,
+          N.land_lor_distr_l, (N.bits_inj_0 (_ .& _)).
+  rewrite N.lor_0_l, <- N.shiftl_lor, <- N.shiftl_land, <- (N.succ_pred (len-i)) by apply N.sub_gt, H.
+  rewrite getmem_succ, 2!N.land_lor_distr_l, 3!N.land_ones, (N.shiftl_mul_pow2 _ Mb).
+  rewrite N.mod_mul, N.lor_0_r by (apply N.pow_nonzero; discriminate).
+  rewrite N.mod_small by apply WTM. reflexivity.
+
+  intro n. rewrite <- N.land_ones, N.land_spec, N.lor_spec, N.land_spec. destruct (N.le_gt_cases (8*i) n).
+    erewrite N.ones_spec_high, (bound_hibits_zero _ (getmem _ _ _ _)), Bool.andb_false_r;
+    [ reflexivity | apply getmem_bound | |]; assumption.
+    rewrite N.shiftl_spec_low by assumption. apply Bool.andb_false_r.
+Qed.
+
+Corollary getbyte:
+  forall i len m a (WTM: welltyped_memory m),
+  i<len -> getmem LittleE len m a .& (N.ones 8 << (8*i)) = m (a+i) << (8*i).
+Proof.
+  intros. rewrite <- (N.lor_0_r (getmem _ _ _ _)).
+  rewrite getbyte_lor by assumption. rewrite N.shiftr_0_l, N.lor_0_r.
+  reflexivity.
+Qed.
+
+Lemma nilfree_extend:
+  forall j m p k (WTM: welltyped_memory m) (P32: p < 2^32) (J4: j <= 4)
+         (NF: nilfree m p (4*k - p mod 4))
+         (NN: forall i, i < j ->
+              (match k with 0 => m Ⓓ[ p - p mod 4 ] .| N.ones (p mod 4 * 8)
+                          | N.pos _ => m Ⓓ[ p - p mod 4 ⊕ 4 * k ]
+               end .& (N.ones 8 << (8*i)) =? 0) = false),
+  nilfree m p (4*k + j - p mod 4).
+Proof.
+  intros. intros i LT. destruct k as [|k].
+
+    rewrite N.add_0_l in LT. rewrite N.mod_small.
+
+      apply N.lt_add_lt_sub_l in LT.
+      specialize (NN _ LT). rewrite getbyte_lor in NN by ((idtac + eapply N.lt_le_trans); eassumption).
+      rewrite N.add_assoc, N.sub_add in NN by (apply N.mod_le; discriminate).
+      intro H. rewrite H in NN. rewrite N.lor_0_l in NN.
+      rewrite shiftr_low_pow2 in NN.
+        rewrite N.mod_0_l, N.shiftl_0_l in NN; [|apply N.pow_nonzero]; discriminate.
+        rewrite N.mul_comm. eapply N.lt_le_trans.
+          apply ones_bound.
+          apply N.pow_le_mono_r. discriminate. apply N.mul_le_mono_l, N.le_add_r.
+
+      rewrite (N.div_mod' p 4). eapply N.lt_le_trans.
+        apply N.add_lt_mono_l. exact LT.
+        rewrite N.add_sub_assoc, N.add_comm, N.add_assoc, N.add_sub, N.add_comm.
+          change (2^32) with (4*N.pred (2^30) + 4). apply N.add_le_mono; [|assumption].
+            apply N.mul_le_mono_l, N.lt_le_pred, N.div_lt_upper_bound, P32. discriminate.
+          intro H. apply N.gt_lt, N.lt_le_incl, N.sub_0_le in H. rewrite H in LT. destruct i; discriminate.
+
+    destruct (N.lt_ge_cases i (4*N.pos k - p mod 4)). apply NF, H.
+    intro H1. assert (H2: p mod 4 <= 4 * N.pos k). transitivity (4*1).
+      apply N.lt_le_incl, N.mod_lt. discriminate.
+      apply N.mul_le_mono_l. destruct k; discriminate.
+    rewrite N.add_sub_swap, N.add_comm, <- (N.sub_add _ _ H) in LT by exact H2.
+    apply N.add_lt_mono_r in LT. specialize (NN _ LT).
+    rewrite getbyte in NN by ((idtac + eapply N.lt_le_trans); eassumption).
+    rewrite <- (N.mod_small (_+_) (2^32)) in NN by (apply index_bound; [|eapply N.lt_le_trans]; eassumption).
+    rewrite N.add_mod_idemp_l in NN by (apply N.pow_nonzero; discriminate).
+    rewrite <- N.add_sub_swap in NN by (apply N.mod_le; discriminate).
+    rewrite <- N.add_sub_assoc, (N.add_sub_assoc _ i) in NN by assumption.
+    rewrite <- (N.add_assoc p), (N.add_comm _ i), (N.add_assoc p), N.add_sub, H1, N.shiftl_0_l in NN.
+    discriminate.
+Qed.
+
+Theorem nilterminate:
+  forall j m p k (WTM: welltyped_memory m) (P32: p < 2^32) (J4: j < 4)
+         (NF: nilfree m p (4*k - p mod 4))
+         (NN: forall i, i < j ->
+              (match k with 0 => m Ⓓ[ p - p mod 4 ] .| N.ones (p mod 4 * 8)
+                          | N.pos _ => m Ⓓ[ p - p mod 4 ⊕ 4 * k ]
+               end .& (N.ones 8 << (8*i)) =? 0) = false)
+         (NIL: (match k with
+                | 0 => m Ⓓ[ p - p mod 4 ] .| N.ones (p mod 4 * 8)
+                | N.pos _ => m Ⓓ[ p - p mod 4 ⊕ 4 * k ]
+                end .& (N.ones 8 << (8*j)) =? 0) = true),
+  nilfree m p (2^32 - p mod 4 ⊕ (4*k + j)) /\
+  m (p ⊕ (2^32 - p mod 4 ⊕ (4*k + j))) = 0.
+Proof.
+  intros. split.
+
+  rewrite <- N.add_sub_swap by (transitivity 4; try apply N.lt_le_incl, N.mod_lt; discriminate).
+  rewrite <- N.add_sub_assoc.
+  rewrite <- N.add_mod_idemp_l, N.mod_same, N.add_0_l by discriminate.
+  apply nilfree_mod.
+  apply nilfree_extend; try apply N.lt_le_incl; assumption.
+  destruct k as [|k].
+
+    rewrite N.add_0_l. intro H. apply N.gt_lt in H.
+    rewrite getbyte_lor, N.mul_comm in NIL by assumption.
+    rewrite N.shiftr_div_pow2, N.ones_div_pow2 in NIL by apply N.mul_le_mono_l, N.lt_le_incl, H.
+    rewrite <- N.mul_sub_distr_l, N.lor_comm in NIL.
+    rewrite N.ones_mod_pow2 in NIL by (change 8 with (8*N.succ 0) at 1;
+      apply N.mul_le_mono_l, N.le_succ_l, N.neq_0_lt_0, N.sub_gt, H).
+    apply Neqb_ok, N.shiftl_eq_0_iff, N.lor_eq_0_l in NIL. discriminate.
+
+    transitivity 4.
+      apply N.lt_le_incl, N.mod_lt. discriminate.
+      etransitivity. apply N.le_add_r. apply N.add_le_mono_r. destruct k; discriminate.
+
+  rewrite N.add_mod_idemp_r, N.add_assoc by discriminate.
+  rewrite N.add_sub_assoc by (transitivity 4; [apply N.lt_le_incl, N.mod_lt|]; discriminate).
+  rewrite (N.add_comm p), <- N.add_sub_assoc by (apply N.mod_le; discriminate).
+  rewrite <- N.add_assoc, <- N.add_mod_idemp_l, N.mod_same, N.add_0_l by discriminate.
+  rewrite N.add_assoc. rewrite <- N.add_mod_idemp_l by discriminate.
+  rewrite N.mod_small by (apply index_bound; assumption).
+  destruct k as [|k].
+
+    rewrite getbyte_lor in NIL by assumption.
+    apply Neqb_ok, N.shiftl_eq_0_iff, N.lor_eq_0_l in NIL.
+    rewrite N.mul_0_r, N.add_0_r, N.mod_small by (eapply N.le_lt_trans; [ apply N.le_sub_l | apply P32 ]).
+    exact NIL.
+
+    rewrite getbyte in NIL by assumption.
+    apply Neqb_ok, N.shiftl_eq_0_iff in NIL. exact NIL.
+Qed.
 
 Theorem strlen_partial_correctness:
-  forall s _r0 lr mem n s' x
-         (HI0: ~ mem_readable s (2^32 - 1)%N)
+  forall s p lr m n s' x
          (MDL0: models armtypctx s)
-         (_R0LO: _r0 < 2^32-3)
-         (_R00: s R_R0 = VaN _r0 32)
-         (LR0: s R_LR = VaN lr 32)
-         (MEM0: s V_MEM32 = VaM mem 32)
+         (MEM0: s V_MEM32 = Ⓜm) (LR0: s R_LR = Ⓓlr) (R0: s R_R0 = Ⓓp)
          (RET: strlen_arm s lr = None)
          (XP0: exec_prog fh strlen_arm 0 s n s' x),
-  trueif_inv (strlen_invset mem _r0 strlen_arm x s').
+  trueif_inv (strlen_invset m p strlen_arm x s').
 Proof.
   intros.
   eapply prove_invs. exact XP0.
-  assumption.
+  exact R0.
   intros.
-  assert (MEM: s1 V_MEM32 = VaM mem 32).
-    rewrite <- MEM0. eapply strlen_preserves_memory. exact XP.
-  assert (HI: ~ mem_readable s1 (2^32 - 1)%N).
-    unfold mem_readable. intro H.
-    destruct H as [r [H1 H2]]. apply HI0. exists r.
-    split; [|exact H2].
-    erewrite <- strlen_preserves_readable; eassumption.
   assert (MDL: models armtypctx s1).
     eapply preservation_exec_prog. exact MDL0. apply strlen_welltyped. exact XP.
-  assert (LR: s1 R_LR = VaN lr 32).
+  assert (MEM: s1 V_MEM32 = Ⓜm).
+    rewrite <- MEM0. eapply strlen_preserves_memory. exact XP.
+  assert (LR: s1 R_LR = Ⓓlr).
     rewrite <- LR0. eapply strlen_preserves_lr. eassumption.
+  assert (WTM := arm_wtm MDL MEM). simpl in WTM.
   rewrite (strlen_nwc s1) in RET.
-  clear s _R00 LR0 HI0 MDL0 MEM0 XP XP0.
-  assert (WTM:=arm_wtm MDL MEM). simpl in WTM.
+  apply (arm_regsize MDL0) in R0. simpl in R0. rename R0 into P32.
+  clear s MDL0 MEM0 LR0 XP XP0.
 
   shelve_cases 32 PRE. Unshelve.
 
   Local Ltac step := time arm_step.
-  2-4: shelve.
-  do 2 step.
-    (* just read 4 bytes, show that this didn't overflow *)
-    assert (LM4: (_r0 .& N.lnot 3 32) + 4 < 2 ^ 32).
-      apply N.lt_nge. intro H. apply HI.
-      replace (_r0 .& N.lnot 3 32) with (2^32-4) in ACC.
-      apply (ACC 3); reflexivity.
-      apply N.le_antisymm.
-        apply N.le_sub_le_add_r. exact H.
-        eapply N.le_trans. eapply and_le_l.
-        replace (2^32-4) with (2^32-3-1) by reflexivity.
-        rewrite <- N.pred_sub.
-        apply N.lt_le_pred. exact _R0LO.
-  do 3 step.
-  (* 0 -> 40, 4-byte aligned, stepped *)
-  apply Neqb_ok, if_true, Neqb_ok in BC; [|discriminate].
-  rename BC into Hmod.
-  (* step all unaligned until 40 since inv proofs are similar *)
-  all: cycle 1.
-  apply N.eqb_neq, if_neq_then, if_false, N.eqb_neq in BC; try discriminate.
-  assert (Hlt: _r0 mod 2^2 < 4) by (apply N.mod_lt; discriminate 1).
-  apply N_lt_4 in Hlt; destruct Hlt as [Hmod|Hmod]; [contradiction|].
 
-  do 3 step.
-    destruct Hmod as [Hmod|[Hmod|Hmod]];
-    try (rewrite Hmod in BC0; discriminate);
-    clear BC BC0.
-  do 2 step.
-  2: rewrite Hmod in BC; discriminate.
-  clear BC tmp tmp0 tmp1.
-
-  all: cycle 1.
-  destruct Hmod as [Hmod|Hmod];
-  try (rewrite Hmod in BC0; discriminate).
-  clear BC BC0.
-
-  do 2 step.
-  1,2: destruct Hmod as [Hmod|Hmod];
-  try (rewrite Hmod in BC; discriminate);
-  clear BC tmp tmp0 tmp1.
-  all: cycle 2.
-  (* at instruction 40, after executing all paths from 0 *)
-  (* goals should be:
-     1. byte aligned
-     2. r0 % 4 = 1 (one byte padded)
-     3. r0 % 4 = 2 (two bytes padded)
-     4. r0 % 4 = 3 (three bytes padded)
-  *)
-  all: exists 0; do 3 eexists;
-       split;[|split;[|split;[|split;[|split]]]];
-       try reflexivity; try assumption.
-  all: right; split; try reflexivity;
-       rewrite N.add_sub, <- mod_and_3.
-  1: split; [left|reflexivity].
-  2: split; [right; left|reflexivity].
-  3: split; [right; right; left|reflexivity].
-  4: split; [right; right; right|reflexivity].
-  all: split; [assumption|].
-  all: reflexivity.
-
-  Unshelve.
-  2-3: shelve.
-  destruct PRE as [n0[r0[r1[r2[R0[R1[R2[R1eq[R1lt Iter]]]]]]]]].
-
+  (* Address 0 *)
+  step. step. step. step.
+    rewrite <- N.ldiff_land_low by (destruct p; [|apply N.log2_lt_pow2;[|apply (arm_regsize MDL PRE)]]; reflexivity).
+    change 3 with (N.ones 2). rewrite ldiff_sub, N.land_ones.
+  step. exists 0.
+    change (2^2) with 4 in *. apply Neqb_ok in BC. rewrite BC. rewrite !N.sub_0_r, N.mul_0_r, N.lor_0_r. repeat split.
+    intros i LT. destruct i; discriminate.
+  step. step.
+    apply N.eqb_neq in BC.
+    assert (LE1: 1 <= p mod 2^2). destruct (p mod _). contradict BC. reflexivity. destruct p0; discriminate.
+    rewrite <- N.add_sub_assoc by exact LE1.
+    rewrite <- (N.add_mod_idemp_l (2^32)), N.mod_same, N.add_0_l by (apply N.pow_nonzero; discriminate).
+    assert (H: p mod 4 - 1 < 2^31). eapply N.le_lt_trans, N.lt_le_trans. apply N.le_sub_l. apply N.mod_lt. discriminate. discriminate.
+    rewrite (N.mod_small (_-1)) by (etransitivity; [exact H | reflexivity]).
+    rewrite shiftr_low_pow2 by exact H. clear H.
+    rewrite modsubcmp by exact LE1.
+  step. step.
+    destruct (p mod 2^2 =? 1) eqn:BC1; [clear BC0|discriminate].
+    apply Neqb_ok in BC1. rewrite BC1, N.sub_diag, N.add_0_r.
+  step. exists 0.
+    change (2^2) with 4 in BC1. rewrite BC1. repeat split.
+    intros i LT. destruct i; discriminate.
   step.
-  step; [apply Neqb_ok, if_false in BC; [| discriminate 1]|].
-  step; [apply Neqb_ok, if_false in BC0; [| discriminate 1]|].
-  step; [apply Neqb_ok, if_false in BC1; [| discriminate 1]|].
-  step; [apply Neqb_ok, if_false in BC2; [| discriminate 1]|].
-  step. 2: rewrite BC2 in BC3; discriminate.
-    (* all 4 bytes nilfree, read 4 bytes *)
-    assert (LM4: r1 + 4 < 2 ^ 32).
-    apply N.lt_nge. intro H. apply HI.
-    replace (2^32-1) with (r1 + (N.pred(2^32) - r1)).
-    apply ACC. apply (N.add_lt_mono_r _ _ r1).
-    rewrite N.sub_add, N.add_comm
-         by apply N.lt_le_pred, (arm_regsize MDL R1).
-    apply N.lt_le_trans with (2^32); [reflexivity | assumption].
-    rewrite N.add_sub_assoc, N.add_comm, N.add_sub
-         by apply N.lt_le_pred, (arm_regsize MDL R1).
-    reflexivity.
-  step. 2: discriminate.
-  clear BC3 BC4 tmp tmp0 tmp1 tmp2 tmp3.
-  (* loops back to 40, all 4 bytes non-nil *)
-  exists (n0+1); do 3 eexists.
-    split;[|split;[|split;[|split;[|split]]]];
-    try reflexivity; try assumption.
-    rewrite N.mul_add_distr_l, N.add_assoc, <- R1eq
-      by discriminate 1.
-    reflexivity.
-    left. split;[|split;[|split;[|split]]].
-    rewrite N.add_comm, N.add_1_l; apply N.neq_succ_0.
-    rewrite N.add_sub; reflexivity.
-    destruct Iter as [[Neq0[HR2[NF[R0lt R0eq]]]]|[Hn0 [Hmod R0eq]]].
-    (* nilfree, show that 4 bytes were checked *)
-    rewrite N.mod_small.
-    apply nilfree_split; [assumption|].
-    unfold nilfree; intros.
-    (* do a whole bunch of rewriting and substitutions *)
-    (* eventually boil down to showing r2 = mem[_r0 + r0] *)
-    apply N.add_cancel_r with (p:=(_r0 .& 3)) in R0eq.
-    rewrite N.sub_add in R0eq
-      by (rewrite <- mod_and_3; replace (2^2) with 4 by reflexivity;
-          apply N.le_trans with 4;
-          [ apply N.lt_le_incl, N.mod_lt; discriminate 1
-          | apply n_lt_mul, N.gt_lt_iff, N.neq_0_lt_0; assumption]).
-    rewrite N.mul_add_distr_l, N.add_assoc, <- R0eq, N.add_assoc in R1eq.
-    rewrite N.add_comm, N.add_shuffle0, <- N.add_comm, N_add_lnot_land_3 in R1eq
-      by (eapply N.lt_trans; [eassumption | reflexivity]).
-    rewrite R1eq, N.add_sub in HR2.
-    (* done rewriting *)
-    subst r2.
-    (* go through each byte, and show it's nilfree *)
-    apply N_lt_4 in H; destruct H as [Hi|[Hi|[Hi|Hi]]]; subst i.
-    (* byte 0 *)
-    rewrite N.add_0_r. rewrite <- N.land_ones in BC.
-    apply N.eqb_neq, N.neq_0_lt_0, N.lt_gt in BC.
-    apply mem_ff_gt0; assumption.
-    (* byte 1 *)
-    apply N.eqb_neq, N.neq_0_lt_0, N.lt_gt in BC0.
-    apply mem_ff00_gt0; assumption.
-    (* byte 2 *)
-    apply N.eqb_neq, N.neq_0_lt_0, N.lt_gt in BC1.
-    apply mem_ff0000_gt0; assumption.
-    (* byte 3 *)
-    apply N.eqb_neq, N.neq_0_lt_0, N.lt_gt in BC2.
-    apply mem_ff000000_gt0; assumption.
-
-    apply N.le_lt_trans with (m:=r1);
-     [ assumption
-     | apply N.lt_trans with (m:=r1+4);
-       [ apply N.lt_add_pos_r; reflexivity
-       | assumption]].
-
-    (* first time looping, some bytes could be padded *)
-    subst n0.
-    simpl (4*(0+1)) in R1eq.
-    rewrite <- mod_and_3 in R0eq by discriminate 1.
-    replace (2^2) with 4 in R0eq by reflexivity.
-    rewrite and_mod_eq, <- mod_and_3 in R1eq
-      by (eapply N.lt_trans; [eassumption | reflexivity]).
-    replace (2^2) with 4 in R1eq by reflexivity.
-    (* check all 4 cases of padding *)
-    destruct Hmod as [[Hmod HR2]|[[Hmod HR2]|[[Hmod HR2]|[Hmod HR2]]]];
-    rewrite Hmod in *.
-    (* no padding, 4-byte aligned *)
-    rewrite N.sub_0_r, N.mod_same in R0eq by discriminate.
-    rewrite N.sub_0_r in R1eq.
-    subst r0 r1.
-    rewrite N.add_sub in HR2.
-    subst r2.
-    rewrite N.add_0_l, N.mod_small by reflexivity.
-    (* essentially identical to just before *)
-    (* show each byte is nilfree *)
-    unfold nilfree; intros.
-    apply N_lt_4 in H; destruct H as [Hi|[Hi|[Hi|Hi]]]; subst i.
-
-    rewrite N.add_0_r. rewrite <- N.land_ones in BC.
-    (* byte 0 *)
-    apply N.eqb_neq, N.neq_0_lt_0, N.lt_gt in BC.
-    apply mem_ff_gt0; assumption.
-    (* byte 1 *)
-    apply N.eqb_neq, N.neq_0_lt_0, N.lt_gt in BC0.
-    apply mem_ff00_gt0; assumption.
-    (* byte 2 *)
-    apply N.eqb_neq, N.neq_0_lt_0, N.lt_gt in BC1.
-    apply mem_ff0000_gt0; assumption.
-    (* byte 3 *)
-    apply N.eqb_neq, N.neq_0_lt_0, N.lt_gt in BC2.
-    apply mem_ff000000_gt0; assumption.
-
-    (* 1 byte padded, _r0 % 4 = 1 *)
-    replace _r0 with (_r0-1+1)
-      by (rewrite N.sub_add; 
-         [ reflexivity
-         | apply mod_n_le with (n:=4); [discriminate|assumption]]).
-    subst r0 r1; rewrite N.add_sub in HR2; subst r2.
-    replace (2 ^ 32 ⊖ 1 ⊕ 4) with 3 by reflexivity.
-    (* show 3 bytes are nilfree *)
-    unfold nilfree; intros.
-    assert (Hi: i < 4) by (eapply N.lt_trans; [eassumption|reflexivity]).
-    apply N_lt_4 in Hi;
-    destruct Hi as [Hi|[Hi|[Hi|Hi]]]; subst i; 
-      try discriminate H; clear H.
-    1-3: rewrite <- N.add_assoc.
-    (* byte 0 *)
-    rewrite N.land_lor_distr_l, N.lor_0_r in BC0.
-    apply N.eqb_neq, N.neq_0_lt_0, N.lt_gt in BC0.
-    apply mem_ff00_gt0; assumption.
-    (* byte 1 *)
-    rewrite N.land_lor_distr_l, N.lor_0_r in BC1.
-    apply N.eqb_neq, N.neq_0_lt_0, N.lt_gt in BC1.
-    apply mem_ff0000_gt0; assumption.
-    (* byte 2 *)
-    rewrite N.land_lor_distr_l, N.lor_0_r in BC2.
-    apply N.eqb_neq, N.neq_0_lt_0, N.lt_gt in BC2.
-    apply mem_ff000000_gt0; assumption.
-
-    (* 2 bytes padded, _r0 % 4 = 2 *)
-    replace _r0 with (_r0-2+2)
-      by (rewrite N.sub_add; 
-         [ reflexivity
-         | apply mod_n_le with (n:=4); [discriminate|assumption]]).
-    subst r0 r1; rewrite N.add_sub in HR2; subst r2.
-    replace (2 ^ 32 ⊖ 2 ⊕ 4) with 2 by reflexivity.
-    (* show 2 bytes are nilfree *)
-    unfold nilfree; intros.
-    assert (Hi: i < 4) by (eapply N.lt_trans; [eassumption|reflexivity]).
-    apply N_lt_4 in Hi;
-    destruct Hi as [Hi|[Hi|[Hi|Hi]]]; subst i; 
-      try discriminate H; clear H.
-    1-2: rewrite <- N.add_assoc.
-    do 2 (rewrite N.land_lor_distr_l, N.lor_0_r in BC1).
-    apply N.eqb_neq, N.neq_0_lt_0, N.lt_gt in BC1.
-    apply mem_ff0000_gt0; assumption.
-
-    do 2 (rewrite N.land_lor_distr_l, N.lor_0_r in BC2).
-    apply N.eqb_neq, N.neq_0_lt_0, N.lt_gt in BC2.
-    apply mem_ff000000_gt0; assumption.
-
-    (* 3 bytes padded, _r0 % 4 = 3 *)
-    replace _r0 with (_r0-3+3)
-      by (rewrite N.sub_add; 
-         [ reflexivity
-         | apply mod_n_le with (n:=4); [discriminate|assumption]]).
-    subst r0 r1; rewrite N.add_sub in HR2; subst r2.
-    replace (2 ^ 32 ⊖ 3 ⊕ 4) with 1 by reflexivity.
-    (* show 1 byte nilfree *)
-    unfold nilfree; intros.
-    assert (Hi: i < 4) by (eapply N.lt_trans; [eassumption|reflexivity]).
-    apply N_lt_4 in Hi;
-    destruct Hi as [Hi|[Hi|[Hi|Hi]]]; subst i; 
-      try discriminate H; clear H.
-
-    rewrite N.add_0_r.
-    do 3 (rewrite N.land_lor_distr_l, N.lor_0_r in BC2).
-    apply N.eqb_neq, N.neq_0_lt_0, N.lt_gt in BC2.
-    apply mem_ff000000_gt0; assumption.
-    (* r0 ⊕ 4 + 4 <= r1 + 4 *)
-    apply N.add_le_mono_r.
-    destruct Iter as [[Hn[HR2[NF[R0lt R0eq]]]]|[Hn[R2eq R0eq]]].
-    rewrite N.mod_small 
-      by (apply N.le_lt_trans with (m:=r1); 
-          [ assumption
-          | apply N.lt_trans with (m:=r1+4); 
-            [ apply N.lt_add_pos_r; reflexivity
-            | assumption]]); assumption.
-    rewrite N.mul_add_distr_l, N.add_assoc, <- N.add_comm in R1eq.
-    subst r0 r1.
-    assert (Hmod: _r0 .& 3 < 4)
-      by (rewrite <- mod_and_3; apply N.mod_lt; discriminate).
-    apply N_lt_4 in Hmod.
-    destruct Hmod as [Hmod|[Hmod|[Hmod|Hmod]]]; rewrite Hmod.
-    1-4: apply N.le_trans with (m:=4); [discriminate | apply N.le_add_r].
-    (* r0 ⊕ 4 = 4 * (n0 + 1) - _r0 mod 2 ^ 2 *)
-    destruct Iter as [[Hn[HR2[NF[R0lt R0eq]]]]|[Hn[R2eq R0eq]]].
-    rewrite N.mod_small.
-    subst r0.
-    rewrite N.mul_add_distr_l, N.add_comm, N.add_sub_assoc,
-            N.add_comm.
-    reflexivity.
-    destruct n0; try contradiction.
-    assert (Hmod: _r0 .& 3 < 4)
-      by (rewrite <- mod_and_3; apply N.mod_lt; discriminate).
-    apply N_lt_4 in Hmod.
-    destruct Hmod as [Hmod|[Hmod|[Hmod|Hmod]]];
-    rewrite Hmod; discriminate.
-    apply N.le_lt_trans with (m:=r1);
-     [ assumption
-     | apply N.lt_trans with (m:=r1+4);
-       [ apply N.lt_add_pos_r; reflexivity
-       | assumption]].
-    subst n0 r0.
-    assert (Hmod: _r0 .& 3 < 4)
-      by (rewrite <- mod_and_3; apply N.mod_lt; discriminate).
-    apply N_lt_4 in Hmod.
-    destruct Hmod as [Hmod|[Hmod|[Hmod|Hmod]]]; rewrite Hmod.
-    1-4: reflexivity.
-
-  (* rest of these cases eventually step to 68 *)
-  (* byte 3 was nil *)
-  apply N.eqb_neq, if_neq_else, if_true in BC2; try discriminate 1.
-  step; [rewrite BC2 in BC3; discriminate | clear BC3].
-  step; [rewrite BC2 in BC3; discriminate | clear BC3].
-  all: cycle 1.
-  (* byte 2 was nil *)
-  apply N.eqb_neq, if_neq_else, if_true in BC1; try discriminate 1.
-  step; [rewrite BC1 in BC2; discriminate | clear BC2].
-  step; [rewrite BC1 in BC2; discriminate | clear BC2].
-  step; [rewrite BC1 in BC2; discriminate | clear BC2].
-  all: cycle 1.
-  (* byte 1 was nil *)
-  apply N.eqb_neq, if_neq_else, if_true in BC0; try discriminate 1.
-  step; [rewrite BC0 in BC1; discriminate | clear BC1].
-  step; [rewrite BC0 in BC1; discriminate | clear BC1].
-  step; [rewrite BC0 in BC1; discriminate | clear BC1].
-  step; [rewrite BC0 in BC1; discriminate | clear BC1].
-  all: cycle 1.
-  (* byte 0 was nil *)
-  apply N.eqb_neq, if_neq_else, if_true in BC; try discriminate 1.
-  step; [rewrite BC in BC0; discriminate | clear BC0].
-  step; [rewrite BC in BC0; discriminate | clear BC0].
-  step; [rewrite BC in BC0; discriminate | clear BC0].
-  step; [rewrite BC in BC0; discriminate | clear BC0].
-  step; [rewrite BC in BC0; discriminate | clear BC0].
-  (* Now at instruction 68 where a nil byte was detected *)
-  (* somewhere in the dword (4 sub-goals)                *)
-  all: exists n0; do 3 eexists;
-       split;[|split;[|split;[|split;[|split;[|split]]]]];
-       try reflexivity; try rewrite mod_and_3; try assumption.
-  all: unfold nilfree_dword; replace 255 with (N.ones 8) by reflexivity;
-       rewrite N.land_ones, BC;
-       try rewrite BC0; try rewrite BC1; try rewrite BC2;
-       reflexivity.
-
-  Unshelve.
-  2: shelve.
-  destruct PRE as [n0[r0[r1[r2[R0[R1[R2[R1eq[R1lt[Iter DW]]]]]]]]]].
-  (* step all paths to 92 *)
-  do 2 step.
-  apply Neqb_ok, if_false in BC; try discriminate 1.
-  step; [clear BC0 | rewrite BC in BC0; discriminate].
-  rewrite <- N.land_ones in BC;
-  replace (N.ones 8) with 255 in BC by reflexivity.
-  step. apply Neqb_ok, if_false in BC0; try discriminate 1.
-  step; [clear BC1 | rewrite BC0 in BC1; discriminate].
-  step. apply Neqb_ok, if_false in BC1; try discriminate 1.
-  clear tmp tmp0 tmp1 tmp2 tmp3 tmp4.
-
-  all: cycle 1.
-  apply N.eqb_neq, if_neq_else, if_true in BC1; try discriminate 1.
-  clear tmp tmp0 tmp1 tmp2 tmp3.
-
-  all: cycle 1.
-  step. discriminate. clear BC0.
-  apply N.eqb_neq, if_neq_else, if_true in BC1; try discriminate 1.
-  step. apply Neqb_ok, if_false in BC0; try discriminate 1.
-  rewrite BC0 in BC1. discriminate.
-  clear BC0 tmp tmp0 tmp1.
-
-  all: cycle 1.
-  step. discriminate. clear BC.
-  apply N.eqb_neq, if_neq_else, if_true in BC0; try discriminate 1.
-  step; [rewrite BC0 in BC; discriminate | clear BC].
-  step; [rewrite BC0 in BC; discriminate | clear BC].
-  step; [rewrite BC0 in BC; discriminate | clear BC].
-  rewrite <- N.land_ones in BC0;
-  replace (N.ones 8) with 255 in BC0 by reflexivity.
-  (* at instruction 92
-     the last byte has either 0, 1, 2, or 3 non-nil bytes before the nil *)
-  all: eexists;
-       split;[|split];
-       try reflexivity; try rewrite <- R1eq; try assumption.
-  (* show that r0 bytes are nilfree *)
-  (* this should put them at the top of the goal list *)
-  all: destruct Iter as [[Hn[HR2[NF[R0lt R0eq]]]]|[Hn[R2eq R0eq]]].
-  (* r2 = [ 00 ?? ?? ?? ] *)
-  (* looped at least once *)
-  assumption.
-  (* didn't loop *)
-  (* must be 4-byte aligned, and first byte is 0 *)
-  subst n0.
-  destruct R2eq as [[Hmod R2eq]|[[Hmod R2eq]|[[Hmod R2eq]|[Hmod R2eq]]]].
-  rewrite <- mod_and_3 in R0eq.
-  replace (2^2) with 4 in R0eq by reflexivity.
-  rewrite Hmod, N.mod_same in R0eq by discriminate.
-  subst r0.
-  unfold nilfree; intros. apply N.nlt_0_r in H. inversion H.
-  (* padded with at least 1 byte, so these 3 cases are contradictions *)
-  1-3: subst r2; apply Neqb_ok in BC0;
-       repeat (
-         rewrite N.land_lor_distr_l, N.lor_comm in BC0;
-         try rewrite N.lor_0_l in BC0);
-       apply N.lor_eq_0_l in BC0; inversion BC0.
-  all: cycle 2.
-  (* looped at least once *)
-  1,5,9: assert (R2val: r2 = mem Ⓓ[ _r0 + r0]).
-  1,3,5: apply N.add_cancel_r with (p:=(_r0 .& 3)) in R0eq; 
-         rewrite N.sub_add in R0eq
-           by (rewrite <- mod_and_3; replace (2^2) with 4 by reflexivity;
-               apply N.le_trans with 4; 
-               [ apply N.lt_le_incl, N.mod_lt; discriminate
-               | apply n_lt_mul, N.gt_lt_iff, N.neq_0_lt_0; assumption]);
-         symmetry in R0eq;
-         rewrite N.mul_add_distr_l, N.add_assoc, R0eq, N.add_assoc in R1eq;
-         rewrite N.add_comm, N.add_shuffle0, <- N.add_comm, N_add_lnot_land_3 in R1eq;
-         rewrite R1eq, N.add_sub in HR2; subst r2; try reflexivity.
-  1-3: eapply N.lt_trans; [eassumption | reflexivity].
-  1-3: clear HR2; subst r2.
-  (* r2 = [ nn nn nn 00 ] *)
-  replace (r0 ⊕ 1 ⊕ 1 ⊕ 1) with (r0 + 3)
-    by (rewrite N.add_mod_idemp_l with (a:=r0 + 1), <- N.add_assoc,
-                N.add_mod_idemp_l, <- N.add_assoc by discriminate;
-        rewrite N.mod_small;
-        [ reflexivity 
-        | apply N.lt_trans with (m:=r0+4);
-          [ apply N.add_lt_mono_l; reflexivity
-          | apply N.le_lt_trans with (m:=r1); assumption ]]).
-  apply nilfree_split; try assumption.
-  unfold nilfree; intros.
-  assert (Hi: i < 4) by (eapply N.lt_trans; [eassumption|reflexivity]).
-  apply N_lt_4 in Hi;
-  destruct Hi as [Hi|[Hi|[Hi|Hi]]]; subst i;
-  try discriminate H; clear H.
-  (* byte 0 nilfree *)
-  rewrite N.add_0_r.
-  apply N.eqb_neq, N.neq_0_lt_0, N.lt_gt in BC.
-  apply mem_ff_gt0; assumption.
-  (* byte 1 nilfree *)
-  apply N.eqb_neq, N.neq_0_lt_0, N.lt_gt in BC0.
-  apply mem_ff00_gt0; assumption.
-  (* byte 2 nilfree *)
-  apply N.eqb_neq, N.neq_0_lt_0, N.lt_gt in BC1.
-  apply mem_ff0000_gt0; assumption.
-
-  (* r2 = [ nn nn 00 ?? ] *)
-  replace (r0 ⊕ 1 ⊕ 1) with (r0 + 2)
-    by (rewrite N.add_mod_idemp_l with (a:=r0 + 1), <- N.add_assoc by discriminate;
-        rewrite N.mod_small;
-        [ reflexivity
-        | apply N.lt_trans with (m:=r0+4);
-          [ apply N.add_lt_mono_l; reflexivity
-          | apply N.le_lt_trans with (m:=r1); assumption ]]).
-  apply nilfree_split; try assumption.
-  unfold nilfree; intros.
-  assert (Hi: i < 4) by (eapply N.lt_trans; [eassumption|reflexivity]).
-  apply N_lt_4 in Hi;
-  destruct Hi as [Hi|[Hi|[Hi|Hi]]]; subst i;
-  try discriminate H; clear H.
-  (* byte 0 nilfree *)
-  rewrite N.add_0_r.
-  apply N.eqb_neq, N.neq_0_lt_0, N.lt_gt in BC.
-  apply mem_ff_gt0; assumption.
-  (* byte 1 nilfree *)
-  apply N.eqb_neq, N.neq_0_lt_0, N.lt_gt in BC0.
-  apply mem_ff00_gt0; assumption.
-
-  (* r2 = [ nn 00 ?? ?? ] *)
-  replace (r0 ⊕ 1) with (r0 + 1)
-    by (rewrite N.mod_small;
-        [ reflexivity
-        | apply N.lt_trans with (m:=r0+4);
-          [ apply N.add_lt_mono_l; reflexivity
-          | apply N.le_lt_trans with (m:=r1); assumption ]]).
-  apply nilfree_split; try assumption.
-  unfold nilfree; intros.
-  apply N.lt_1_r in H; subst i.
-  (* byte 0 nilfree *)
-  rewrite N.add_0_r.
-  apply N.eqb_neq, N.neq_0_lt_0, N.lt_gt in BC.
-  apply mem_ff_gt0; assumption.
-
-  (* didn't loop, so string < 4 bytes *)
-  1,4,7: subst n0.
-  replace (r0 ⊕ 1 ⊕ 1 ⊕ 1) with (r0 ⊕ 3)
-    by (rewrite N.add_mod_idemp_l with (a:=r0 + 1), <- N.add_assoc,
-                N.add_mod_idemp_l, <- N.add_assoc by discriminate;
-                reflexivity).
-  rewrite and_mod_eq, <- mod_and_3 in R1eq
-    by (eapply N.lt_trans; [eassumption | reflexivity]).
-  replace (2^2) with 4 in R1eq by reflexivity.
-  simpl (4*(0+1)) in R1eq.
-  destruct R2eq as [[Hmod R2eq]|[[Hmod R2eq]|[[Hmod R2eq]|[Hmod R2eq]]]];
-  rewrite <- mod_and_3 in R0eq; replace (2^2) with 4 in R0eq by reflexivity;
-  rewrite Hmod in R0eq by discriminate;
-  subst r0.
-  1: replace (2 ^ 32 ⊖ 0 ⊕ 3) with 3 by reflexivity.
-  2: replace (2 ^ 32 ⊖ 1 ⊕ 3) with 2 by reflexivity.
-  3: replace (2 ^ 32 ⊖ 2 ⊕ 3) with 1 by reflexivity.
-  4: replace (2 ^ 32 ⊖ 3 ⊕ 3) with 0 by reflexivity.
-  1-4: rewrite Hmod in *; subst r1; rewrite N.add_sub in R2eq;
-       try rewrite N.sub_0_r in R2eq; subst r2.
-  (* 4-byte aligned *)
-  unfold nilfree; intros.
-  assert (Hi: i < 4) by (eapply N.lt_trans; [eassumption|reflexivity]).
-  apply N_lt_4 in Hi;
-  destruct Hi as [Hi|[Hi|[Hi|Hi]]]; subst i;
-    try discriminate H; clear H.
-
-  rewrite N.add_0_r.
-  apply N.eqb_neq, N.neq_0_lt_0, N.lt_gt in BC.
-  apply mem_ff_gt0; assumption.
-  apply N.eqb_neq, N.neq_0_lt_0, N.lt_gt in BC0.
-  apply mem_ff00_gt0; assumption.
-  apply N.eqb_neq, N.neq_0_lt_0, N.lt_gt in BC1.
-  apply mem_ff0000_gt0; assumption.
-
-  (* 1 byte padded *)
-  replace _r0 with (_r0-1+1)
-    by (rewrite N.sub_add; 
-         [ reflexivity
-         | apply mod_n_le with (n:=4); [discriminate|assumption]]).
-  unfold nilfree; intros.
-  assert (Hi: i < 4) by (eapply N.lt_trans; [eassumption|reflexivity]).
-  apply N_lt_4 in Hi;
-  destruct Hi as [Hi|[Hi|[Hi|Hi]]]; subst i; 
-    try discriminate H; clear H.
-
-  rewrite N.add_0_r. rewrite N.land_lor_distr_l, N.lor_0_r in BC0.
-  apply N.eqb_neq, N.neq_0_lt_0, N.lt_gt in BC0.
-  apply mem_ff00_gt0; assumption.
-
-  rewrite N.land_lor_distr_l, N.lor_0_r in BC1.
-  rewrite <- N.add_assoc.
-  apply N.eqb_neq, N.neq_0_lt_0, N.lt_gt in BC1.
-  apply mem_ff0000_gt0; assumption.
-  (* 2 bytes padded *)
-  replace _r0 with (_r0-2+2)
-    by (rewrite N.sub_add; 
-         [ reflexivity
-         | apply mod_n_le with (n:=4); [discriminate|assumption]]).
-  unfold nilfree; intros.
-  assert (Hi: i < 4) by (eapply N.lt_trans; [eassumption|reflexivity]).
-  apply N_lt_4 in Hi;
-  destruct Hi as [Hi|[Hi|[Hi|Hi]]]; subst i; 
-    try discriminate H; clear H.
-
-  rewrite N.add_0_r.
-  rewrite N.land_lor_distr_l, N.lor_0_r,
-          N.land_lor_distr_l, N.lor_0_r in BC1.
-  apply N.eqb_neq, N.neq_0_lt_0, N.lt_gt in BC1.
-  apply mem_ff0000_gt0; assumption.
-  (* 3 bytes padded *)
-  unfold nilfree; intros. apply N.nlt_0_r in H. inversion H.
-
-  replace (r0 ⊕ 1 ⊕ 1) with (r0 ⊕ 2).
-  2: rewrite N.add_mod_idemp_l, <- N.add_assoc by discriminate 1;
-       simpl (1+1); reflexivity.
-  rewrite and_mod_eq, <- mod_and_3 in R1eq; replace (2^2) with 4 in R1eq by reflexivity.
-  2: eapply N.lt_trans; [eassumption | reflexivity].
-  destruct R2eq as [[Hmod R2eq]|[[Hmod R2eq]|[[Hmod R2eq]|[Hmod R2eq]]]];
-  rewrite <- mod_and_3 in R0eq; replace (2^2) with 4 in R0eq by reflexivity;
-  rewrite Hmod in R0eq by discriminate;
-  subst r0.
-  4:{ subst r2; apply Neqb_ok in BC1.
-      rewrite N.land_lor_distr_l, N.lor_comm in BC1.
-      apply N.lor_eq_0_l in BC1. inversion BC1. }
-  1: replace (2 ^ 32 ⊖ 0 ⊕ 2) with 2 by reflexivity.
-  2: replace (2 ^ 32 ⊖ 1 ⊕ 2) with 1 by reflexivity.
-  3: replace (2 ^ 32 ⊖ 2 ⊕ 2) with 0 by reflexivity.
-  1-3: simpl (4*(0+1)) in R1eq;
-       rewrite Hmod in *; subst r1; rewrite N.add_sub in R2eq.
-  (* %4 = 0 *)
-  rewrite N.sub_0_r in R2eq. subst r2.
-  unfold nilfree; intros.
-  assert (Hi: i < 4). eapply N.lt_trans; [eassumption|reflexivity].
-    apply N_lt_4 in Hi;
-    destruct Hi as [Hi|[Hi|[Hi|Hi]]]; subst i;
-      try discriminate H; clear H.
-
-  rewrite N.add_0_r.
-  apply N.eqb_neq, N.neq_0_lt_0, N.lt_gt in BC.
-  apply mem_ff_gt0; assumption.
-
-  apply N.eqb_neq, N.neq_0_lt_0, N.lt_gt in BC0.
-  apply mem_ff00_gt0; assumption.
-
-  (* %4  = 1 *)
-  replace _r0 with (_r0-1+1).
-  2:{ rewrite N.sub_add. reflexivity. apply mod_n_le with (n:=4); [discriminate|assumption]. }
-  unfold nilfree; intros.
-  subst r2.
-  assert (Hi: i < 4). eapply N.lt_trans; [eassumption|reflexivity].
-  apply N_lt_4 in Hi;
-  destruct Hi as [Hi|[Hi|[Hi|Hi]]]; subst i; 
-    try discriminate H; clear H.
-
-  rewrite N.add_0_r. rewrite N.land_lor_distr_l, N.lor_0_r in BC0.
-  apply N.eqb_neq, N.neq_0_lt_0, N.lt_gt in BC0.
-  apply mem_ff00_gt0; assumption.
-
-  unfold nilfree; intros. apply N.nlt_0_r in H. inversion H.
-
-  rewrite and_mod_eq, <- mod_and_3 in R1eq; replace (2^2) with 4 in R1eq by reflexivity.
-  2: eapply N.lt_trans; [eassumption | reflexivity].
-  destruct R2eq as [[Hmod R2eq]|[[Hmod R2eq]|[[Hmod R2eq]|[Hmod R2eq]]]];
-  rewrite <- mod_and_3 in R0eq; replace (2^2) with 4 in R0eq by reflexivity;
-  rewrite Hmod in R0eq by discriminate;
-  subst r0.
-  3:{ subst r2; apply Neqb_ok in BC1.
-      rewrite N.land_lor_distr_l, N.lor_comm in BC1.
-      apply N.lor_eq_0_l in BC1. inversion BC1. }
-  3:{ subst r2; apply Neqb_ok in BC1.
-      rewrite N.land_lor_distr_l, N.lor_comm,
-          N.lor_0_l, N.land_lor_distr_l, N.lor_comm in BC1.
-      apply N.lor_eq_0_l in BC1. inversion BC1. }
-  1: replace (2 ^ 32 ⊖ 0 ⊕ 1) with 1 by reflexivity.
-  2: replace (2 ^ 32 ⊖ 1 ⊕ 1) with 0 by reflexivity.
-  1-2: simpl (4*(0+1)) in R1eq;
-       rewrite Hmod in *; subst r1; rewrite N.add_sub in R2eq.
-  (* %4 = 0 *)
-  rewrite N.sub_0_r in R2eq. subst r2.
-  unfold nilfree; intros.
-  assert (Hi: i < 4). eapply N.lt_trans; [eassumption|reflexivity].
-    apply N_lt_4 in Hi;
-    destruct Hi as [Hi|[Hi|[Hi|Hi]]]; subst i;
-      try discriminate H; clear H.
-
-  rewrite N.add_0_r.
-  apply N.eqb_neq, N.neq_0_lt_0, N.lt_gt in BC.
-  apply mem_ff_gt0; assumption.
-
-  (* %4  = 1 *)
-  unfold nilfree; intros. apply N.nlt_0_r in H. inversion H.
-
-  (* show last byte is nil *)
-  (* looped *)
-  1,3,5,7: assert (R2val: r2 = mem Ⓓ[ _r0 + r0]).
-  1,3,5,7: apply N.add_cancel_r with (p:=(_r0 .& 3)) in R0eq; 
-           rewrite N.sub_add in R0eq
-           by (rewrite <- mod_and_3; replace (2^2) with 4 by reflexivity;
-               apply N.le_trans with 4; 
-               [ apply N.lt_le_incl, N.mod_lt; discriminate
-               | apply n_lt_mul, N.gt_lt_iff, N.neq_0_lt_0; assumption]);
-           symmetry in R0eq;
-       rewrite N.mul_add_distr_l, N.add_assoc, R0eq, N.add_assoc in R1eq;
-       simpl (4*1) in R1eq;
-       rewrite N.add_comm, N.add_shuffle0, <- N.add_comm, N_add_lnot_land_3 in R1eq;
-       rewrite R1eq, N.add_sub in HR2; subst r2; try reflexivity.
-  1-4: eapply N.lt_trans; [eassumption | reflexivity].
-  1-4: clear HR2; subst r2.
-
-  unfold nilfree_dword in DW. rewrite BC, BC0, BC1 in DW.
-  destruct (mem Ⓓ[ _r0 + r0] .& 4278190080 =? 0) eqn:BC2; try discriminate.
-  apply Neqb_ok in BC2.
-  replace (r0 ⊕ 1 ⊕ 1 ⊕ 1) with (r0 + 3).
-  2: rewrite N.add_mod_idemp_l with (a:=r0 + 1), <- N.add_assoc,
-          N.add_mod_idemp_l, <- N.add_assoc by discriminate 1;
-       simpl (1+1+1);
-       rewrite N.mod_small;
-       [ reflexivity 
-       | apply N.lt_trans with (m:=r0+4);
-         [ apply N.add_lt_mono_l; reflexivity
-         | apply N.le_lt_trans with (m:=r1); assumption ]].
-  rewrite N.add_assoc. apply mem_ff000000_eq0 in BC2; assumption.
-
-  replace (r0 ⊕ 1 ⊕ 1) with (r0 + 2).
-  2: rewrite N.add_mod_idemp_l with (a:=r0 + 1), <- N.add_assoc by discriminate;
-       simpl (1+1); 
-       rewrite N.mod_small;
-       [ reflexivity
-       | apply N.lt_trans with (m:=r0+4);
-         [ apply N.add_lt_mono_l; reflexivity
-         | apply N.le_lt_trans with (m:=r1); assumption ]].
-  rewrite N.add_assoc.
-  apply Neqb_ok in BC1.
-  apply mem_ff0000_eq0 in BC1; assumption.
-
-  replace (r0 ⊕ 1) with (r0 + 1).
-  2: rewrite N.mod_small;
-     [ reflexivity
-     | apply N.lt_trans with (m:=r0+4);
-       [ apply N.add_lt_mono_l; reflexivity
-       | apply N.le_lt_trans with (m:=r1); assumption ]].
-  rewrite N.add_assoc.
-  apply Neqb_ok in BC1.
-  apply mem_ff00_eq0 in BC1; assumption.
-
-  apply Neqb_ok in BC0.
-  apply mem_ff_eq0 in BC0; assumption.
-
-  (* didn't loop *)
-  all: subst n0; rewrite and_mod_eq, <- mod_and_3, N.mul_add_distr_l, N.add_assoc in R1eq;
-       replace (2^2) with 4 in R1eq by reflexivity;
-       simpl (4*(0+1)) in R1eq.
-  2,4,6,8: eapply N.lt_trans; [eassumption | reflexivity].
-  all: cycle -1.
-  destruct R2eq as [[Hmod R2eq]|[[Hmod R2eq]|[[Hmod R2eq]|[Hmod R2eq]]]].
-  rewrite <- mod_and_3 in R0eq. replace (2^2) with 4 in R0eq by reflexivity.
-  rewrite Hmod, N.mod_same in R0eq by discriminate.
-  subst r0. rewrite Hmod, N.sub_0_r in R1eq.
-  subst r1. rewrite N.add_sub in R2eq.
-  subst r2.
-  rewrite N.add_0_r. rewrite N.add_0_r in BC0.
-  apply Neqb_ok in BC0. apply mem_ff_eq0 in BC0; assumption.
-
-  1-3: subst r2; apply Neqb_ok in BC0.
-
-  rewrite N.land_lor_distr_l, N.lor_comm in BC0.
-  apply N.lor_eq_0_l in BC0. inversion BC0.
-
-  rewrite N.land_lor_distr_l, N.lor_comm,
-          N.lor_0_l, N.land_lor_distr_l, N.lor_comm in BC0.
-  apply N.lor_eq_0_l in BC0. inversion BC0.
-
-  rewrite N.land_lor_distr_l, N.lor_comm,
-          N.lor_0_l, N.land_lor_distr_l, N.lor_comm,
-          N.lor_0_l, N.land_lor_distr_l, N.lor_comm in BC0.
-  apply N.lor_eq_0_l in BC0. inversion BC0.
-
-  replace (r0 ⊕ 1 ⊕ 1 ⊕ 1) with (r0 ⊕ 3).
-  2: rewrite N.add_mod_idemp_l with (a:=r0 + 1), <- N.add_assoc,
-          N.add_mod_idemp_l, <- N.add_assoc by discriminate 1;
-       simpl (1+1+1); reflexivity.
-
-  destruct R2eq as [[Hmod R2eq]|[[Hmod R2eq]|[[Hmod R2eq]|[Hmod R2eq]]]];
-  rewrite <- mod_and_3 in R0eq; replace (2^2) with 4 in R0eq by reflexivity;
-  rewrite Hmod in R0eq by discriminate;
-  subst r0.
-  1: replace (2 ^ 32 ⊖ 0 ⊕ 3) with 3 by reflexivity.
-  2: replace (2 ^ 32 ⊖ 1 ⊕ 3) with 2 by reflexivity.
-  3: replace (2 ^ 32 ⊖ 2 ⊕ 3) with 1 by reflexivity.
-  4: replace (2 ^ 32 ⊖ 3 ⊕ 3) with 0 by reflexivity.
-  1-4: rewrite Hmod in *; subst r1; rewrite N.add_sub, N.add_0_r in R2eq.
-  (* %4 = 0 *)
-  rewrite N.sub_0_r in R2eq.
-  1-4: subst r2; unfold nilfree_dword in DW; rewrite BC, BC0, BC1 in DW.
-  destruct (mem Ⓓ[ _r0] .& 4278190080 =? 0) eqn:BC2; try discriminate.
-  apply Neqb_ok in BC2. apply mem_ff000000_eq0 in BC2; assumption.
-
-  replace _r0 with (_r0-1+1).
-  2:{ rewrite N.sub_add. reflexivity. apply mod_n_le with (n:=4); [discriminate|assumption]. }
-  destruct (mem Ⓓ[ _r0 - 1 ] .| 255 .& 4278190080 =? 0) eqn:BC2; try discriminate.
-  apply Neqb_ok in BC2.
-  rewrite N.land_lor_distr_l, N.lor_comm, N.lor_0_l in BC2.
-  rewrite <- N.add_assoc.
-  apply mem_ff000000_eq0 in BC2; assumption.
-
-  replace _r0 with (_r0-2+2).
-  2:{ rewrite N.sub_add. reflexivity. apply mod_n_le with (n:=4); [discriminate|assumption]. }
-  destruct (mem Ⓓ[ _r0 - 2] .| 255 .| 65280 .& 4278190080 =? 0) eqn:BC2; try discriminate.
-  apply Neqb_ok in BC2.
-  rewrite N.land_lor_distr_l, N.lor_comm, N.lor_0_l,
-          N.land_lor_distr_l, N.lor_comm, N.lor_0_l in BC2.
-  rewrite <- N.add_assoc.
-  apply mem_ff000000_eq0 in BC2; assumption.
-
-  replace _r0 with (_r0-3+3).
-  2:{ rewrite N.sub_add. reflexivity. apply mod_n_le with (n:=4); [discriminate|assumption]. }
-  destruct (mem Ⓓ[ _r0 - 3] .| 255 .| 65280 .| 16711680 .& 4278190080 =? 0) eqn:BC2; try discriminate.
-  apply Neqb_ok in BC2.
-  rewrite N.land_lor_distr_l, N.lor_comm, N.lor_0_l,
-          N.land_lor_distr_l, N.lor_comm, N.lor_0_l,
-          N.land_lor_distr_l, N.lor_comm, N.lor_0_l in BC2.
-  rewrite <- N.add_assoc.
-  apply mem_ff000000_eq0 in BC2; assumption.
-
-  replace (r0 ⊕ 1 ⊕ 1) with (r0 ⊕ 2).
-  2: rewrite N.add_mod_idemp_l, <- N.add_assoc by discriminate 1;
-       simpl (1+1); reflexivity.
-
-  destruct R2eq as [[Hmod R2eq]|[[Hmod R2eq]|[[Hmod R2eq]|[Hmod R2eq]]]];
-  rewrite <- mod_and_3 in R0eq; replace (2^2) with 4 in R0eq by reflexivity;
-  rewrite Hmod in R0eq by discriminate;
-  subst r0.
-  4:{ subst r2. apply Neqb_ok in BC1.
-      rewrite N.land_lor_distr_l, N.lor_comm in BC1.
-      apply N.lor_eq_0_l in BC1. inversion BC1. }
-  1: replace (2 ^ 32 ⊖ 0 ⊕ 2) with 2 by reflexivity.
-  2: replace (2 ^ 32 ⊖ 1 ⊕ 2) with 1 by reflexivity.
-  3: replace (2 ^ 32 ⊖ 2 ⊕ 2) with 0 by reflexivity.
-  1-3: rewrite Hmod in *; subst r1; rewrite N.add_sub, N.add_0_r in R2eq.
-  (* %4 = 0 *)
-  rewrite N.sub_0_r in R2eq.
-  1-3: subst r2; apply Neqb_ok in BC1. 
-  apply mem_ff0000_eq0 in BC1; assumption.
-
-  replace _r0 with (_r0-1+1).
-  2:{ rewrite N.sub_add. reflexivity. apply mod_n_le with (n:=4); [discriminate|assumption]. }
-  rewrite N.land_lor_distr_l, N.lor_comm, N.lor_0_l in BC1.
-  rewrite <- N.add_assoc.
-  apply mem_ff0000_eq0 in BC1; assumption.
-
-  replace _r0 with (_r0-2+2).
-  2:{ rewrite N.sub_add. reflexivity. apply mod_n_le with (n:=4); [discriminate|assumption]. }
-  rewrite N.land_lor_distr_l, N.lor_comm, N.lor_0_l,
-          N.land_lor_distr_l, N.lor_comm, N.lor_0_l in BC1.
-  rewrite <- N.add_assoc.
-  apply mem_ff0000_eq0 in BC1; assumption.
-
-  destruct R2eq as [[Hmod R2eq]|[[Hmod R2eq]|[[Hmod R2eq]|[Hmod R2eq]]]];
-  rewrite <- mod_and_3 in R0eq; replace (2^2) with 4 in R0eq by reflexivity;
-  rewrite Hmod in R0eq by discriminate;
-  subst r0.
-  3:{ subst r2. apply Neqb_ok in BC1.
-      rewrite N.land_lor_distr_l, N.lor_comm in BC1.
-      apply N.lor_eq_0_l in BC1. inversion BC1. }
-  3:{ subst r2. apply Neqb_ok in BC1.
-      rewrite N.land_lor_distr_l, N.lor_comm, N.lor_0_l,
-              N.land_lor_distr_l, N.lor_comm in BC1.
-      apply N.lor_eq_0_l in BC1. inversion BC1. }
-  1: replace (2 ^ 32 ⊖ 0 ⊕ 1) with 1 by reflexivity.
-  2: replace (2 ^ 32 ⊖ 1 ⊕ 1) with 0 by reflexivity.
-  1-2: rewrite Hmod in *; subst r1; rewrite N.add_sub in R2eq.
-  (* %4 = 0 *)
-  rewrite N.sub_0_r, N.add_0_r in R2eq.
-  1-2: subst r2; apply Neqb_ok in BC1.
-  apply mem_ff00_eq0 in BC1; assumption.
-
-  replace _r0 with (_r0-1+1).
-  2:{ rewrite N.sub_add. reflexivity. apply mod_n_le with (n:=4); [discriminate|assumption]. }
-  rewrite N.land_lor_distr_l, N.lor_comm, N.lor_0_l, N.add_0_r in BC1.
-  rewrite <- N.add_assoc.
-  apply mem_ff00_eq0 in BC1; assumption.
-
-  Unshelve.
-  destruct PRE as [r0[R0[NF LB]]].
+    destruct (p mod 2^2 =? 1) eqn:BC1; [discriminate|clear BC0]. apply N.eqb_neq in BC1.
+    assert (LE2: 1 <= p mod 2 ^ 2 - 1). destruct (p mod 2^2). contradict BC;reflexivity. repeat (discriminate + (contradict BC1;reflexivity) + destruct p1).
+    rewrite <- N.add_sub_assoc by exact LE2.
+    rewrite <- (N.add_mod_idemp_l (2^32)), N.mod_same, N.add_0_l by (apply N.pow_nonzero; discriminate).
+    assert (H: p mod 4 - 1 - 1 < 2^31). eapply N.le_lt_trans, N.le_lt_trans, N.lt_le_trans; try (apply N.mod_lt + apply N.le_sub_l); discriminate.
+    rewrite (N.mod_small (_-1)) by (etransitivity; [exact H | reflexivity]).
+    rewrite shiftr_low_pow2 by exact H. clear H.
+    rewrite 2!modsubcmp by (exact LE1 + exact LE2).
   step.
-  unfold strlen_post.
-  exists r0. split; [|split].
-  rewrite update_frame by discriminate 1; assumption.
-  assumption. assumption.
+    exists 0. destruct (p mod 2^2 =? 1 + 1) eqn:BC2; [clear BC0|discriminate].
+      apply Neqb_ok in BC2. change (2^2) with 4 in *. rewrite BC2, <- N.lor_assoc. repeat split.
+      intros i LT. destruct i; discriminate.
+    exists 0. change (2^2) with 4 in *. replace (p mod 4) with 3.
+      rewrite <- !N.lor_assoc. repeat split. intros i LT. destruct i; discriminate.
+      assert (LT3: p mod 4 < 4). apply N.mod_lt. discriminate.
+      destruct (p mod 4). contradict BC; reflexivity. repeat (discriminate + destruct p2). reflexivity. exfalso. apply LE2. reflexivity.
+
+  (* Address 40 *)
+  destruct PRE as [k [R0 [R1 [R2 NF]]]].
+  step. step.
+
+    (* nil at offset 4k+0 *)
+    repeat (discriminate + step). eexists. simpl_stores. split.
+      rewrite <- (N.add_0_r (4*k)). reflexivity.
+      rewrite <- N.land_ones in BC5. apply nilterminate; try assumption. reflexivity.
+      intros i LT. destruct i; discriminate.
+
+    (* nil at offset 4k+1 *)
+    step. repeat (discriminate + step). eexists. simpl_stores. split.
+      repeat rewrite N.add_mod_idemp_l, <- N.add_assoc by discriminate. reflexivity.
+      rewrite <- N.land_ones in BC5. apply nilterminate; try assumption. reflexivity.
+      intros i LT. destruct i as [|i]. assumption. repeat (discriminate LT + assumption + destruct i as [i|i|]).
+
+    (* nil at offset 4k+2 *)
+    step. repeat (discriminate + step). eexists. simpl_stores. split.
+      repeat rewrite N.add_mod_idemp_l, <- N.add_assoc by discriminate. reflexivity.
+      rewrite <- N.land_ones in BC5. apply nilterminate; try assumption. reflexivity.
+      intros i LT. destruct i as [|i]. assumption. repeat (discriminate LT + assumption + destruct i as [i|i|]).
+
+    (* nil at offset 4k+3 *)
+    step. repeat (discriminate + step). eexists. simpl_stores. split.
+      repeat rewrite N.add_mod_idemp_l, <- N.add_assoc by discriminate. reflexivity.
+      rewrite <- N.land_ones in BC5. apply nilterminate; try assumption. reflexivity.
+      intros i LT. destruct i as [|i]. assumption. repeat (discriminate LT + assumption + destruct i as [i|i|]).
+
+    (* no nils from 4k+0 to 4k+3: iterate loop *)
+    repeat (step; [|discriminate]). exists (N.succ k). repeat split.
+      rewrite N.mul_succ_r, N.add_assoc, N.add_mod_idemp_l by (apply N.pow_nonzero; discriminate). reflexivity.
+      rewrite (N.mul_succ_r _ (N.succ _)), N.add_assoc, N.add_mod_idemp_l by (apply N.pow_nonzero; discriminate). reflexivity.
+      destruct (N.succ k) eqn:H. destruct k; discriminate. reflexivity.
+
+      rewrite N.mul_succ_r. apply nilfree_extend; try (assumption + reflexivity).
+      intros i LT. rewrite <- N.land_ones in BC.
+      destruct i as [|i]. assumption. repeat (discriminate LT + assumption + destruct i as [i|i|]).
 Qed.
